---
dg-home: false
dg-publish: true
---
# Anti-derivatives

1) Use [[3.1 Antiderivatives#^b5075f|integration by parts]] to compute the anti-derivatives of the following functions
	$$ \begin{split} 1) \qquad & f(x) = x^{2}\,(x +1)^{9} \\ & \\ 2) \qquad & f(x) = x^{2}(2x - 1)^{-7} \\ & \\ 3) \qquad & f(x) = \ln(x) \\ & \\ 4)  \qquad & f(x) = x\ln(x) \\ & \\ 5)  \qquad & f(x) = (\ln(x))^{2} \\ & \\ 6)  \qquad & f(x) = \arcsin(x) \\ & \\ 7)  \qquad & f(x) = \arccos(x) \\ & \\ 8)  \qquad & f(x) = \arctan(x) \\ & \\ 9)  \qquad & f(x) = \mathrm{e}^{x}\,\sin(x)\\ & \\ 10)  \qquad & f(x) = x^{3} \,\sin(x^{2})\\ & \\ 11)  \qquad & f(x) = x\,\ln(x+1)\\ & \\ 12)  \qquad & f(x) = x\,\sqrt{x+1}\\ & \\ 13) \qquad & f(x) = \cos(\ln(x))\qquad \mbox{Hint: integrate by parts twice} \\ & \\ 14) \qquad & f(x) = \frac{1}{x}\arcsin(\ln(x)) \\ & \\ 15) \qquad & f(x) = x\,\arctan(x^{2}) \\ & \\ \end{split} $$

2) If $f\colon[a,b]\rightarrow \mathbb{R}$ is continuous and invertible in $(a,b)$ with inverse $f^{-1}$ and primitive $F$, use [[3.1 Antiderivatives#^b5075f|integration by parts]] to prove that 
	$$ \int f^{-1}(x)\,\mathrm{d}x =x f^{-1}(x) - F(f^{-1}(x)) + c .$$

3) Use the [[3.1 Antiderivatives#^93db8a|a suitable change of variable]] to compute the anti-derivatives of the following functions
	$$ \begin{split} 1) \qquad & f(x) = \frac{1 + \sqrt{1-\sqrt{x}}}{\sqrt{x}}  \\ & \\ 2) \qquad & f(x) =  x^{2}\,\sin(\sqrt{x^{3}}) \\ & \\ 3) \qquad & f(x) =   \cos(\ln(x)) \\ & \\ 4) \qquad & f(x) =   \frac{\sqrt{x}+1}{x+3} \\ & \\ 5) \qquad & f(x) =  \frac{x^{3}}{(1+x^{2})^{3}} \\ & \\ 6) \qquad & f(x) =   \frac{1}{(x+2)\sqrt{1+x}} \\ & \\ 7) \qquad & f(x) =   \frac{\mathrm{e}^{4x}}{\mathrm{e}^{2x} + 2\mathrm{e}^{x} + 2} \\ & \\ 8) \qquad & f(x) =   \frac{1}{\sqrt{\mathrm{e}^{2x} - 1}}\\ & \\ 9) \qquad & f(x) =   \frac{\sin^{2}(x)\,\cos^{5}(x)}{\tan^{3}(x)}\\ & \\ 10) \qquad & f(x) =  \frac{\sin(x) + 3\cos(x)}{\sin(x) + 2\cos(x)} \\ & \\ 11) \qquad & f(x) =   \frac{\sin(x) + 3\cos(x)}{\sin(x)\cos(x) + \sin(x)}\\ & \\ 12) \qquad & f(x) = \sqrt{\sqrt{x} + 1}  \\ & \\ 13) \qquad & f(x) = \frac{1}{\mathrm{e}^{x} - 4\mathrm{e}^{-x}} \\ & \\ 14) \qquad & f(x) = \frac{1}{x^{2}\sqrt{9-x^{2}}}  \\ & \\ \end{split} $$
	>[!note]- Solution:
	>1) Use $t=\sqrt{1-\sqrt{x}}$.
	>2) Use $t=x^{\frac{3}{2}}$.
	>3) Use $t=\ln(x)$ and integrate by part twice.
	>4) Use $t=\sqrt{x} +1$ and long division of polynomials.
	>5) Use $t=1+x^2$.
	>6) Use $t=\sqrt{1+x}$.
	>7) Use $t=\mathrm{e}^x$ and long division of polynomials.
	>8) Use $t=\sqrt{\mathrm{e}^{2x}-1}$.
	>9) Use $t=\cos(x)$. 
	>10) Use
	>11) Use $t=\tan(x/2)$, so that $\sin(x)=2t/(1+t^2)$ and $\cos(x)=(1-t)/(1+t^2)$. 
	>12) Use $t=\sqrt{\sqrt{x}+1}$.
	>13) Use $t=\mathrm{e}^x$.
	>14) Use first $y=x/3$ and then $y=\sin(t)$. 

# Double integrals 

1) Compute the double integral
	$$ \iint_{D}y^{2}\,\mathrm{d}A$$
	where $D$ is the triangular region with vertices $(0,2)$, $(2,4)$, and $(4,2)$.

2) Compute the double integral
	$$ \iint_{D}\mathrm{e}^{x-y}\,\mathrm{d}A $$
	where $D$ is the triangular region with vertices $(0,0)$, $(1,3)$, and $(2,2)$.

3) Compute the following double integrals and sketch the regions of integration:
	$$ \begin{split} 1) \qquad & \int_{0}^{2}\int_{\frac{x}{8}}^{\sqrt[3]{x}}\, \;\mathrm{d}y\,\mathrm{d}x & \\ 2) \qquad & \int_{1}^{2}\int_{\ln(x)}^{\mathrm{e}^{x}}\, \;\mathrm{d}y\,\mathrm{d}x & \\ 3) \qquad & \int_{0}^{2}\int_{2}^{3}\, (x + \mathrm{e}^{-y})\;\mathrm{d}x\,\mathrm{d}y & \\ 4)  \qquad & \int_{1}^{3}\int_{\frac{\pi}{2}}^{\pi}\,y\sin(x) \;\mathrm{d}x\,\mathrm{d}y & \\ 5)  \qquad & \int_{2}^{3}\int_{1}^{4}\,\left(\frac{x}{y} + \frac{y}{x}\right) \;\mathrm{d}y\,\mathrm{d}x & \\ 6)  \qquad & \int_{0}^{\frac{\pi}{2}}\int_{0}^{y}\, y\sin(x)\;\mathrm{d}x\,\mathrm{d}y & \\ 7)  \qquad & \int_{0}^{1}\int_{0}^{x}\,\sqrt{1-x^{2}} \;\mathrm{d}y\,\mathrm{d}x & \\ 8)  \qquad & \int_{0}^{3}\int_{0}^{x^{2}}\,y^{2}x \;\mathrm{d}y\,\mathrm{d}x & \\ 9)  \qquad & \int_{0}^{1}\int_{x}^{1}\,xy \;\mathrm{d}y\,\mathrm{d}x & \\ 10)  \qquad & \int_{0}^{\frac{\pi}{2}}\int_{0}^{\cos(x)}\,\cos(x) \;\mathrm{d}y\,\mathrm{d}x & \\ 11)  \qquad & \int_{-1}^{1}\int_{|y|}^{1}\,(x+y)^{2} \;\mathrm{d}x\,\mathrm{d}y & \\ 12)  \qquad & \int_{-3}^{1}\int_{-\sqrt{9-y^{2}}}^{\sqrt{9-y^{2}}}\, x^{2}\;\mathrm{d}x\,\mathrm{d}y & \\ 13) \qquad & \int_{-1}^{1}\int_{-2|x|}^{|x|}\,\mathrm{e}^{x+y} \;\mathrm{d}y\,\mathrm{d}x & \\ 14) \qquad & \int_{0}^{1}\int_{2-y}^{1}\,(x+y)^{2} \;\mathrm{d}x\,\mathrm{d}y & \\ 15) \qquad & \int_{0}^{1}\int_{1}^{\mathrm{e}^{x}}\,x + y \;\mathrm{d}y\,\mathrm{d}x \end{split} $$

4) Compute the following integrals by changing the order of integration:
	$$ \begin{split} 1) \qquad & \int_{0}^{a }\int_{0}^{\sqrt{a^{2} - x^{2}}}\sqrt{a^{2} - y^{2}}\, \;\mathrm{d}y\,\mathrm{d}x & \\ 2)  \qquad & \int_{1}^{2}\int_{0}^{\ln(x)}\,(x-1)\,\sqrt{1+ \mathrm{e}^{2y}} \;\mathrm{d}y\,\mathrm{d}x & \\ 3)  \qquad & \int_{0}^{8}\int_{\frac{y}{2}}^{4}\, \;\mathrm{d}x\,\mathrm{d}y & \\ 4)  \qquad & \int_{0}^{1}\int_{x}^{1}\,xy \;\mathrm{d}y\,\mathrm{d}x & \\ 5)  \qquad & \int_{-3}^{1}\int_{-\sqrt{9-y^{2}}}^{\sqrt{9-y^{2}}}x^{2}\, \;\mathrm{d}x\,\mathrm{d}y & \\ 6)  \qquad & \int_{0}^{4}\int_{\frac{y}{2}}^{2}\,\mathrm{e}^{x^{2}} \;\mathrm{d}x\,\mathrm{d}y & \\ 7)  \qquad & \int_{0}^{3}\int_{\sqrt[3]{x}}^{27}\,xy \;\mathrm{d}y\,\mathrm{d}x \end{split} $$
	>[!note]- Solution:
	>1)
	>2) The region of integration reads $D=\{(x,y)\in\mathbb{R}^{2}|1\leq x\leq 2, 0\leq y\leq \ln(x)\}$. As such, it is written as a $y$-simple region, but we can turn it into an $x$-simple region writing $D=\{(x,y)\in\mathbb{R}^{2}|0\leq y\leq \ln(2),\mathrm{e}^{y}\leq x\leq 2\}$. Next, we perform the change of variable $\mathrm{e}^{y}=t$, which means $\mathrm{e}^{y}\mathrm{d}y=\mathrm{d}t$ and thus
	>	$$\begin{split} \int_{1}^{2}\int_{0}^{\ln(x)}(x-1)\sqrt{1+\mathrm{e}^{2y}}\,\mathrm{d}y\mathrm{d}x&=\int_{0}^{\ln(2)}\int_{\mathrm{e}^{y}}^{2}(x-1)\sqrt{1+\mathrm{e}^{2y}}\,\mathrm{d}x\mathrm{d}y=\\ &= \int_{0}^{\ln(2)}\mathrm{e}^{y}\left(1-\frac{\mathrm{e}^{y}}{2}\right)\sqrt{1+\mathrm{e}^{2y}}\,\mathrm{d}y= \\ &=\int_{1}^{2}\left(1-\frac{t}{2}\right)\sqrt{1+t^{2}}\,\mathrm{d}t=\\ & =\int_{1}^{2} \sqrt{1+t^{2}}\,\mathrm{d}t-\int_{1}^{2}\frac{t}{2}\sqrt{1+t^{2}}\,\mathrm{d}t.\end{split}$$
	>	The second integral is immediate because $2t$ is the derivative of $1+t^{2}$, and the result is thus $\frac{1}{6}(2^{\frac{3}{2}}-5^{\frac{3}{2}})$. To solve the first integral in the RHS of the previous long chain of equalities, we introduce the change of variable $t=\sinh(u)$ (look [here](https://en.wikipedia.org/wiki/Hyperbolic_functions) for the definition and all the properties of hyperbolic functions we need), which leads to $\mathrm{d}t=\cosh(x)\mathrm{d}u$ and $1+\sinh^{2}(u)=\cosh^{2}(u)$. Since $\cosh(u)$ is always positive, we have
	>	$$\begin{split}\int_{1}^{2} \sqrt{1+t^{2}}\,\mathrm{d}t&=\int_{0}^{\mathrm{arcsinh}(2)} \cosh^{2}(u)\,\mathrm{d}u= \\ & =\int_{0}^{\mathrm{arcsinh}(2)}\cosh(u) \cosh(u)\,\mathrm{d}u= \\ & = \sinh(x)\cosh(x) - \int_{0}^{\mathrm{arcsinh}(2)} \sinh^{2}(u)\,\mathrm{d}u=\\ & =\sinh(x)\cosh(x) - \int_{0}^{\mathrm{arcsinh}(2)} \cosh^{2} (u)-1\,\mathrm{d}u,\end{split}$$
	>	which leads to
	>	$$\begin{split}\int_{0}^{\mathrm{arcsinh}(2)}\cosh^{2}(u)\,\mathrm{d}u&=\left[\frac{sinh(u)\cosh(u) +u}{2}\right]_{0}^{\mathrm{arcsinh}(2)}=\\ &= \cosh(\mathrm{arcsinh}(2))+\frac{\mathrm{arcsinh(2)}}{2}\end{split}.$$
	>	In conclusion, the original integral is $cosh(\mathrm{arcsinh}(2))+\frac{\mathrm{arcsinh(2)}}{2}+\frac{1}{6}(2^{\frac{3}{2}}-5^{\frac{3}{2}})$. 
	>3)
	>4)
	>5)
	>6)
	>7)


# Double integrals and change of variables

1) Let $D$ be the closed unit disk in $\mathbb{R}^{2}$. Compute the double integral
	$$ \iint_{D}\mathrm{e}^{x^2 + y^{2}}\;\mathrm{d}A$$
	using a suitable change of variables.

2) Let $D$ be the region in $\mathbb{R}^{2}$ delimited by the lines
	$$ x+y=0,\quad x+y=1,\quad 2x-y=0,\quad 2x-y=3 . $$
	Compute the double integral
	$$ \iint_{D}(x^{2} + y^{2})\;\mathrm{d}A $$
	using a suitable change of variables.

3) Let $D$ be the region in $\mathbb{R}^2$ delimited by
	$$ x^2 + y^2 = 4,\quad  x^2 + y^2 = 9, \quad x^2 - y^2 = 1, \quad x^{2 }- y^{2} = 4.$$
	Compute the double integral 
	$$ \iint_{D}xy\;\mathrm{d}A $$
	using a suitable change of variable.

4) Consider the region
	$$ D=\left\lbrace (x,y)\in \mathbb{R}^2 \mid x\geq 2,\: (x-2)^2+y^{2}\leq 1 \right\rbrace . $$
	Using the polar coordinates transformation with center at the point $(1,0)$ shows that $D$ is the image of a simple region in the plane $(r,\theta)$. Compute the double integral 
	$$ \iint_D \dfrac{1}{x-1}\,dA\,, $$
	exploiting the change of variable just discussed.
	>[!note]- Solution:
	>The transformation reads
	>$$(r,\theta)\mapsto (x=1+r\cos\theta , y= r\sin\theta),$$
	>	and the determinant of its jacobian is $r$ like in the case of ordinary polar coordinates. In this coordinates, the inequality $x\geq 2$ becomes $r\cos\theta\geq 1$, while the inequality $(x-2)^2+y^{2}\leq 1$ becomes $r^{2}\cos^{2}(\theta) - 2r\cos\theta + 1+ r^{2}\sin^{2}(\theta)\leq 1$, which means $r\leq 2\cos\theta$. Consequently, the region $D$ is the image of the region $D^{*}$ determined by $\frac{1}{\cos\theta}\leq r\leq 2\cos\theta$, and $0\leq \theta \leq \frac{\pi}{4}$. The inequality in $\theta$ follows from drawing the region $D$ in the $xy$-plane, and recalling the geometrical interpretation of the angle theta for the generalized polar coordinates introduced above. Clearly, the region $D^{*}$ is $r$-simple, and so it is an elementary region in the $r\theta$-plane. Applying the change of variable formula, the integral becomes
	>	$$\iint_{D}\frac{1}{x-1}\mathrm{d}A=\iint_{D^{*}}\frac{r}{r\cos\theta}\mathrm{d}A'=\int_{0}^{\frac{\pi}{4}}\int_{\frac{1}{\cos\theta}}^{2\cos\theta}\frac{1}{\cos\theta}\mathrm{d}r\,\mathrm{d}\theta=[2\theta - \tan\theta]_{0}^{\frac{\pi}{4}}=\frac{\pi}{2} -1$$

5) Evaluate the double integral: 
	$$ I = \int_{0}^{\pi/2}\int_{0}^{2\sin(\theta)}\frac{r\sqrt{1+\sin^{2}(\theta)}}{\sin(\theta)}\,\mathrm{d}r\,\mathrm{d}\theta$$
	  >[!note]- Solution:
	  >We first evaluate the inner integral with respect to $r$ because we can treat $\theta$ as a constant for this step:
	  >$$ \int_{0}^{2\sin(\theta)}\frac{r\sqrt{1+\sin^{2}(\theta)}}{\sin(\theta)}\,\mathrm{d}r = \frac{\sqrt{1+\sin^{2}(\theta)}}{\sin(\theta)} \left[ \frac{r^{2}}{2} \right]_{r=0}^{r=2\sin(\theta)}= 2\sin(\theta)\,\sqrt{1+\sin^{2}(\theta)},$$
	  >where we used that $\sin(\theta)\neq0$ for $\theta\in(0,\frac{\pi}{2}$], and that the potential issue at $\theta=0$ where $\sin(0)=0$ is handled because the result of the inner definite integral correctly evaluates to $0$ at $\theta=0$. To evaluate the outer integral
	  >$$I = \int_{0}^{\frac{\pi}{2}} 2\sin(\theta)\sqrt{1+\sin^{2}(\theta)}\,\mathrm{d}\theta,$$
	  >we use the substitution $u=\cos(\theta)$, from which we obtain  $\sin^{2}(\theta)=1−\cos^{2}(\theta)=1−u^{2}$, and $\mathrm{d}u=−\sin(\theta)\mathrm{d}\theta$, so that the change of the limits of variable leads to
	  >$$ I = \int_{1}^{0} 2 \sqrt{1+(1-u^2)} (-\mathrm{d}u)  = \int_{1}^{0} -2 \sqrt{2-u^{2},\mathrm{d}u}= \int_{0}^{1} 2 \sqrt{2-u^2},\mathrm{d}u.$$
	  >This integral requires a trigonometric substitution. Let $u=\sqrt{2}\sin(\phi)$. Then $\mathrm{d}u=\sqrt{2}\cos(\phi)\mathrm{d}\phi$, $\phi\in[0,\pi/4]$, and
	  >$$ I = \int_{0}^{\pi/4} 2 \sqrt{2(1 - \sin^2(\phi))} (\sqrt{2}\cos(\phi))\,\mathrm{d}\phi = \int_{0}^{\pi/4} 2 \sqrt{2\cos^2(\phi)} (\sqrt{2}\cos(\phi))\,\mathrm{d}\phi   = \int_{0}^{\pi/4} 4\cos^2(\phi)\,\mathrm{d}\phi,$$
	  >where we used $1−\sin^{2}(\phi)=\cos^{2}(\phi)$, and the fact that $0\leq\phi\leq\frac{\pi}{4}$ implies $\cos(\phi)\geq 0$, and $\sqrt{\cos^{2}(\phi)}=\cos(\phi)$.  Using the identity $cos^{2}(\phi)=\frac{1+\cos(\phi)}{2}$​, we obtain
	  >$$ I = \int_{0}^{\pi/4} 4 \left( \frac{1+\cos(2\phi)}{2} \right)\,\mathrm{d}\phi = 2 \int_{0}^{\pi/4} (1+\cos(2\phi))\,\mathrm{d}\phi= 2 \left[ \phi + \frac{\sin(2\phi)}{2} \right]_{0}^{\pi/4} =  \boxed{1 + \frac{\pi}{2}}.$$

# Triple integrals

1)  Evaluate the following triple integral
	$$ \iiint_{W} \sin(x)\,\mathrm{d}V $$
	where $W$ is the solid given by $0\leq x\leq \pi$, $0,\leq y\leq 1$, $0, z\leq x$.

2) Let $W$ be the region bounded by the planes $x=0$, $y = 0$, and $z=2$, and the surface $z = x^{2} + y^{2}$, and lying in the quadrant $x \geq 0$, $y\geq  0$. Compute 
	$$ \iiint_{W}x\,\mathrm{d}V $$
	in two different ways, and sketch the region $W$.

3) Evaluate the triple integral
	$$ \iiint_{W}\,\mathrm{d}V=\int_{0}^{1}\int_{0}^{x}\int_{x^{2} + y^{2}}^{2}\,\mathrm{d}z\,\mathrm{d}y \,\mathrm{d}x, $$
	sketch the region $W$ and interpret the result geometrically.
